Fix extraction for case study #2. WIP some admits.

io/case-studies/IO_Sig_Call.ml
@@ -1,7 +1,7 @@
 open Prims
 open Common
 open FStar_Pervasives
-open Free_IO
+open IO_Sig
 
 let ml_call (cmd:io_cmds) =
   match cmd with
@@ -31,4 +31,7 @@ let io_call (cmd:io_cmds) argz =
 let (iio_call : inst_cmds -> Obj.t -> Obj.t iio) =
   fun cmd -> fun argz ->
   match cmd with
-  | GetTrace -> iio_return (Obj.magic (Monitor.get_trace ()))
+  | GetTrace -> 
+    print_string "Getting trace...\n";
+    flush stdout;
+    iio_return (Obj.magic (Monitor.get_trace ()))
