io/TC.MLify.IIOwp.fst
@@ -15,6 +15,23 @@ open DM.IIO
 
 exception Something_went_really_bad
  
+let rec skip_partial_calls (tree:dm_iio 'a (trivial_hist ())) : ML 'a =
+  match tree with
+  | Return y -> y
+  | PartialCall pre k -> begin
+    assume (trivial_hist () `hist_ord` dm_iio_theta tree); //by (norm [delta_only [`%dm_iio;`%DMFree.dm;`%dm_iio_theta]]; dump "H");
+    assert (forall p h. trivial_hist #'a #event () p h);
+    assert (forall p h. dm_iio_theta tree p h);
+    assert (forall p h. dm_iio_theta tree p h ==> pre);
+    admit ();
+    skip_partial_calls (k ())
+  end
+  (** during extraction, Free.IO.Call is replaced with an actual
+  implementation of the commands, therefore, the `Call` constructor
+  does not exist **)
+  | _ -> FStar.All.raise Something_went_really_bad
+
+
 instance mlifyable_iiowp
   t1 t2 {| ml t1 |} {| ml t2 |} :
   Tot (mlifyable (t1 -> IIOwp t2 (trivial_hist ()))) =
@@ -22,13 +39,8 @@ instance mlifyable_iiowp
     #(t1 -> IIOwp t2 (trivial_hist ()))
     (t1 -> ML t2)
     (fun f x -> 
-     let tree : iio t2 = reify (f x) in
-     match tree with
-     | Return y -> y
-     (** during extraction, Free.IO.Call is replaced with an actual
-     implementation of the commands, therefore, the `Call` constructor
-     does not exist **)
-     | _ -> FStar.All.raise Something_went_really_bad)
+     let tree : dm_iio t2 (trivial_hist ()) = reify (f x) in
+     skip_partial_calls tree)
 
 (** Ideas to improve mlifyable_iio_miio:
 1. What if instead of Tot, we use Ex, to be able to internalize try_catch.
@@ -52,10 +64,5 @@ instance mlifyable_inst_iiowp
     (d1.start_type -> ML t3)
     #(ml_ml_arrow_1 d1.start_type t3 #d1.start_type_c #d2)
     (fun (p:t1 -> IIOwp t3 (trivial_hist ())) (ct:d1.start_type) ->
-     let tree : iio t3 = reify (p (d1.instrument ct)) in
-     match tree with
-     | Return y -> y
-     (** during extraction, Free.IO.Call is replaced with an actual
-     implementation of the commands, therefore, the `Call` constructor
-     does not exist **)
-     | _ -> FStar.All.raise Something_went_really_bad)
+     let tree : dm_iio t3 (trivial_hist ()) = reify (p (d1.instrument ct)) in
+     skip_partial_calls tree)
