io/case-studies/Utils.fst
@@ -43,3 +43,25 @@ effect IOpi
     (fun p h ->
       pre h /\
       (forall r lt. (io_post pi h r lt /\ post h r lt) ==> p lt r))
+
+let _IIOwp_as_MIIO
+  (pre:'a -> trace -> bool)
+  (post:'a -> trace -> (m:'b) -> trace -> Type0)
+  (f:(x:'a ->
+    IIOwp 'b (fun p h -> pre x h /\ (forall r lt. post x h r lt ==> p lt r))))
+  (x:'a) :
+  IIOwp (Common.maybe 'b) (trivial_hist ()) =
+  (trivialize 
+    #_ 
+    #(trivializeable_IIOwp _ _ (fun x h -> pre x h) post) f) x
+
+let _IIOwp_as_MIIO_2
+  (pre:'a -> 'b -> trace -> bool)
+  (post:'a -> 'b -> trace -> (m:'c) -> trace -> Type0)
+  (f:(x:'a -> y:'b ->
+    IIOwp 'c (fun p h -> pre x y h /\ (forall r lt. post x y h r lt ==> p lt r))))
+  (x:'a) (y:'b):
+  IIOwp (Common.maybe 'c) (trivial_hist ()) =
+  (trivialize 
+    #_ 
+    #(trivializeable_IIOwp_2 _ _ _ (fun x y h -> pre x y h) post) f) x y
